fixed typing! When converting types, we ask the 2 types to be convertible

theories/LambdaCube/Typing.v
@@ -46,8 +46,8 @@ Inductive typing (P: pi_scheme) : forall {n}, typing_ctx n -> term n -> term n -
   Γ ⊢(P) Abs A t : Pi A B
 | typ_app {n} {Γ: typing_ctx n} {A B t u} :
   Γ ⊢(P) t : Pi A B -> Γ ⊢(P) u : A -> Γ ⊢(P) App t u : bind (bind_first u) B
-| typ_conv {n} {Γ: typing_ctx n} {t A B} :
-  Γ ⊢(P) t : A -> A ≅ B -> Γ ⊢(P) t : B
+| typ_conv {n} {Γ: typing_ctx n} {t A B s} :
+  Γ ⊢(P) t : A -> A ≅ B -> Γ ⊢(P) B : Srt s -> Γ ⊢(P) t : B
 with ctx_wf (P: pi_scheme) : forall {n}, typing_ctx n -> Prop :=
 | empty_wf : \ ⊢(P)
 | cons_wf {n} {A: typing_ctx n} {t: term n} {s} :
@@ -112,7 +112,7 @@ Lemma typ_var_inv Sc {n} (Γ : typing_ctx n) i T :
   (Γ ⊢(Sc) Var i : T) -> T ≅ kth_index_ctx Γ (proj1_sig i) (proj2_sig i).
   remember (Var i). induction 1 in i, Heqt |- *; try discriminate.
   - inversion Heqt. subst. constructor.
-  - subst. specialize (IHtyping _ eq_refl). eapply Requiv_trans; eauto using Requiv_sym.
+  - subst. specialize (IHtyping1 _ eq_refl). eapply Requiv_trans; eauto using Requiv_sym.
 Qed.
 
 Lemma typ_pi_inv Sc {n} (Γ : typing_ctx n) A B T :
@@ -121,23 +121,23 @@ Lemma typ_pi_inv Sc {n} (Γ : typing_ctx n) A B T :
 Proof.
   remember (Pi A B). induction 1 in A, B, Heqt |- *; try discriminate.
   - exists s. exists s'. inversion Heqt; subst; clear Heqt. intuition constructor.
-  - subst. specialize (IHtyping _ _ eq_refl). destruct IHtyping as [s [s']].
-    exists s. exists s'. intuition. eauto using Requiv_trans, Requiv_sym.
+  - subst. specialize (IHtyping1 _ _ eq_refl). destruct IHtyping1 as [s0 [s']].
+    exists s0. exists s'. intuition. eauto using Requiv_trans, Requiv_sym.
 Qed.
 
 Lemma typ_abs_inv Sc {n} (Γ: typing_ctx n) A t T :
   Γ ⊢(Sc) Abs A t : T ->
-  exists s s' B,
+  exists s s' B X,
     T ≅ Pi A B /\ Γ ⊢(Sc) A : Srt s /\ Γ, A ⊢(Sc) B : Srt s' /\ Γ, A ⊢(Sc) t : B /\
-      pi_scheme_check Sc s s'.
+      Γ ⊢(Sc) T : X /\ pi_scheme_check Sc s s'.
 Proof.
   remember (Abs A t).
   induction 1 in A, t, Heqt0 |- *; try discriminate.
   - clear IHtyping1 IHtyping2 IHtyping3. inversion Heqt0. subst. clear Heqt0.
-    exists s. exists s'. exists B. intuition constructor.
-  - subst. specialize (IHtyping A t eq_refl).
-    destruct IHtyping as [s [s' [B0]]].
-    exists s. exists s'. exists B0. intuition eauto using Requiv_trans, Requiv_sym.
+    exists s. exists s'. exists B. exists (Srt s'). intuition econstructor; eassumption.
+  - subst. specialize (IHtyping1 A t eq_refl).
+    destruct IHtyping1 as [s0 [s' [B0]]].
+    exists s0, s', B0, (Srt s). firstorder eauto using Requiv_trans, Requiv_sym.
 Qed.
 
 Lemma typ_app_inv Sc {n} (Γ: typing_ctx n) t u T :
@@ -146,8 +146,8 @@ Proof.
   remember (App t u) as t0.
   induction 1 in t, u, Heqt0 |- *; try discriminate.
   - clear IHtyping1 IHtyping2. exists A, B. inversion Heqt0; subst; clear Heqt0. intuition constructor.
-  - subst. specialize (IHtyping _ _ eq_refl).
-    destruct IHtyping as [A0 [B0]].
+  - subst. specialize (IHtyping1 _ _ eq_refl).
+    destruct IHtyping1 as [A0 [B0]].
     exists A0, B0. intuition eauto using Requiv_trans, Requiv_sym.
 Qed.
 
@@ -156,33 +156,7 @@ Proof.
   induction 1; try assumption.
 Qed.
 
-Lemma equiv_context (Sc : pi_scheme) {n} (Γ Γ': typing_ctx n) t s :
-  (forall k H, kth_index_ctx Γ' k H ≅ kth_index_ctx Γ k H) -> Γ' ⊢(Sc) -> Γ ⊢(Sc) t : s -> Γ' ⊢(Sc) t : s.
-Proof.
-  intros H pr. induction 1.
-  - constructor. assumption.
-  - econstructor; swap 1 2. { apply H. } constructor. assumption.
-  - econstructor; try eassumption; auto.
-    apply IHtyping2.
-    + intros. simpl. destruct (lt_dec k n); try solve [constructor].
-      apply ren_preserves_step_equiv. auto.
-    + econstructor; try eassumption.
-      apply IHtyping1; assumption.
-  - econstructor; try eassumption; auto.
-    + apply IHtyping2.
-      * intros. simpl. destruct (lt_dec k n); try solve [constructor].
-        apply ren_preserves_step_equiv. auto.
-      * econstructor; try eassumption.
-        apply IHtyping1; assumption.
-    + apply IHtyping3.
-      * intros. simpl. destruct (lt_dec k n); try solve [constructor].
-        apply ren_preserves_step_equiv. auto.
-      * econstructor; try assumption. apply IHtyping1; assumption.
-  - econstructor; auto.
-  - econstructor; eauto.
-Qed.
-
-Lemma weakening {Sc n k} {σ: {i | i < n} -> {i | i < k}} {Γ Γ' x T}  :
+Lemma gen_weakening {Sc n k} {σ: {i | i < n} -> {i | i < k}} {Γ Γ' x T}  :
   (forall i,
       ren σ (kth_index_ctx Γ (proj1_sig i) (proj2_sig i)) =
         kth_index_ctx Γ' (proj1_sig (σ i)) (proj2_sig (σ i))) ->
@@ -236,126 +210,304 @@ Lemma weakening {Sc n k} {σ: {i | i < n} -> {i | i < k}} {Γ Γ' x T}  :
         destruct (lt_dec _ _); try tauto. f_equal. apply sig_lt_ext. reflexivity.
       * simpl. destruct (lt_dec _ _); try lia. reflexivity.
   - econstructor.
-    + apply IHtyping; assumption.
+    + apply IHtyping1; assumption.
     + apply ren_preserves_step_equiv. assumption.
+    + apply IHtyping2; assumption.
+Qed.
+
+Lemma weakening {Sc n} {Γ: typing_ctx n} {A x T s}:
+  Γ ⊢(Sc) x : T -> Γ ⊢(Sc) A : Srt s -> Γ, A ⊢(Sc) ren weaken x : ren weaken T.
+Proof.
+  intros. eapply gen_weakening; eauto.
+  - destruct i; simpl. destruct (lt_dec _ _); try tauto. f_equal. f_equal. apply le_unique.
+  - econstructor; try eassumption. eapply typing_imp_ctx_wf; eassumption.
+Qed.
+
+Lemma wf_ctx_contains_types {Sc n} {Γ : typing_ctx n} {k l} :
+  Γ ⊢(Sc) -> exists s, Γ ⊢(Sc) kth_index_ctx Γ k l : Srt s.
+  induction 1 in k, l |- *; simpl.
+  - destruct (Nat.nlt_0_r _ _).
+  - destruct (lt_dec _ _).
+    + edestruct IHctx_wf as [s']. change (Srt ?s) with (ren (@weaken n) (Srt s)).
+      eexists. eapply weakening; eassumption.
+    + exists s. change (Srt s) with (ren (@weaken n) (Srt s)). eapply weakening; eassumption.
+Qed.
+
+Lemma equiv_context (Sc : pi_scheme) {n} (Γ Γ': typing_ctx n) t s :
+  (forall k H, kth_index_ctx Γ' k H ≅ kth_index_ctx Γ k H) ->
+  (forall k H, exists s, Γ' ⊢(Sc) kth_index_ctx Γ k H : Srt s) ->
+  Γ' ⊢(Sc) -> Γ ⊢(Sc) t : s -> Γ' ⊢(Sc) t : s.
+Proof.
+  intros H Htyp pr. induction 1.
+  - constructor. assumption.
+  - edestruct Htyp. econstructor; swap 1 2; try eassumption.
+    + apply H.
+    + constructor. assumption.
+  - econstructor; try eassumption; auto.
+    apply IHtyping2.
+    + intros. simpl. destruct (lt_dec k n); try solve [constructor].
+      apply ren_preserves_step_equiv. auto.
+    + simpl. intros. destruct (lt_dec _ _).
+      * edestruct Htyp as [s0]. exists s0. change (@Srt (S ?n) ?x) with (ren weaken (@Srt n x)).
+        eapply weakening; eauto.
+      * exists s. change (@Srt (S n) s) with (ren weaken (@Srt n s)). eapply weakening; eauto.
+    + econstructor; try eassumption.
+      apply IHtyping1; assumption.
+  - econstructor; try eassumption; auto.
+    + apply IHtyping2.
+      * intros. simpl. destruct (lt_dec k n); try solve [constructor].
+        apply ren_preserves_step_equiv. auto.
+      * intros. simpl. destruct (lt_dec _ _).
+        -- edestruct Htyp as [s0]. exists s0. change (@Srt (S ?n) ?x) with (ren weaken (@Srt n x)).
+           eapply weakening; try eassumption.
+           apply IHtyping1; assumption.
+        -- exists s. change (@Srt (S ?n) ?x) with (ren weaken (@Srt n x)).
+           eapply weakening; apply IHtyping1; assumption.
+      * econstructor; try eassumption.
+        apply IHtyping1; assumption.
+    + apply IHtyping3.
+      * intros. simpl. destruct (lt_dec k n); try solve [constructor].
+        apply ren_preserves_step_equiv. auto.
+      * intros. simpl. destruct (lt_dec _ _).
+        -- edestruct Htyp as [s0]. exists s0. change (@Srt (S ?n) ?x) with (ren weaken (@Srt n x)).
+           eapply weakening; try eassumption.
+           apply IHtyping1; assumption.
+        -- exists s. change (@Srt (S ?n) ?x) with (ren weaken (@Srt n x)).
+           eapply weakening; apply IHtyping1; assumption.
+      * econstructor; try assumption. apply IHtyping1; assumption.
+  - econstructor; auto.
+  - econstructor; eauto.
+Qed.
+
+Lemma bind_typ Sc n k (σ : {i | i < k} -> term n) Γ Γ' x T :
+          (forall i, Γ ⊢(Sc) σ i : bind σ (kth_index_ctx Γ' (proj1_sig i) (proj2_sig i))) ->
+          Γ' ⊢(Sc) x : T -> Γ ⊢(Sc) -> Γ ⊢(Sc) bind σ x : bind σ T.
+  intros H tyx Γwf. induction tyx in n, σ, Γ, H, Γwf |- *; simpl in *; auto.
+  - constructor. assumption.
+  - econstructor; eauto. eapply IHtyx2.
+    + intro. unfold lift_bind at 1. destruct (lt_dec _ _).
+      * rewrite bind_weaken. eapply weakening; eauto.
+      * rewrite bind_weaken.
+        replace (ren weaken (bind σ A)) with
+          (kth_index_ctx (Γ, bind σ A) n (Nat.lt_succ_diag_r n)).
+        -- constructor. econstructor; eauto.
+        -- simpl. destruct (lt_dec n n); try lia. reflexivity.
+    + econstructor; eauto.
+  - econstructor; eauto.
+    + apply IHtyx2.
+      * intro. rewrite bind_weaken. unfold lift_bind.
+        destruct (lt_dec _ _).
+        -- eapply weakening; eauto.
+        -- replace (ren weaken (bind σ A)) with
+             (kth_index_ctx (Γ, bind σ A) n (Nat.lt_succ_diag_r n)).
+           ++ do 2 econstructor; eauto.
+           ++ simpl. destruct (lt_dec _ _); try lia. reflexivity.
+      * econstructor; eauto.
+    + apply IHtyx3.
+      * intro. rewrite bind_weaken. unfold lift_bind at 1. destruct (lt_dec _ _).
+        -- eapply weakening; eauto.
+        -- replace (ren weaken (bind σ A)) with
+             (kth_index_ctx (Γ, bind σ A) n (Nat.lt_succ_diag_r n)).
+           ++ do 2 econstructor; eauto.
+           ++ simpl. destruct (lt_dec _ _); try lia. reflexivity.
+      * econstructor; eauto.
+  - rewrite bind_comp. replace (bind (bind σ ∘ bind_first u) B) with
+      (bind (bind_first (bind σ u)) (bind (lift_bind σ) B)).
+    + econstructor; eauto.
+    + rewrite bind_comp. apply bind_ext. intro. unfold lift_bind, bind_first at 2.
+      destruct (lt_dec _ _); simpl.
+      * rewrite bind_ren. apply bind_id. intro. unfold weaken, bind_first. simpl.
+        pose proof (proj2_sig k). simpl in *. destruct (lt_dec _ _); try tauto.
+        f_equal. apply sig_lt_ext. reflexivity.
+      * unfold bind_first. simpl. destruct (lt_dec _ _); try lia. reflexivity.
+  - econstructor; eauto. apply bind_preserves_step_equiv. assumption.
+Qed.
+
+Lemma typed_imp_subterm_typed {Sc} {n k} {Γ u T} {K: ctx k n} :
+  Γ ⊢(Sc) fill K u : T -> exists Γ' T', Γ' ⊢(Sc) u : T'.
+  remember (fill K u) as t. induction 1 in k, u, K, Heqt |- *.
+  - destruct K; simpl in *; try discriminate. subst.
+    do 2 eexists. constructor. eassumption.
+  - destruct K; simpl in *; try discriminate. subst. do 2 eexists. constructor. eassumption.
+  - destruct K; simpl in *; try discriminate.
+    + subst. do 2 eexists. econstructor; eassumption.
+    + inversion Heqt. eauto.
+    + inversion Heqt. eauto.
+  - destruct K; simpl in *; try discriminate.
+    + subst. do 2 eexists. econstructor; eassumption.
+    + inversion Heqt. eauto.
+    + inversion Heqt. eauto.
+  - destruct K; simpl in *; try discriminate.
+    + subst. do 2 eexists. econstructor; eassumption.
+    + inversion Heqt. eauto.
+    + inversion Heqt. eauto.
+  - eauto.
+Qed.
+
+Lemma unique_typing {n Sc Γ} {t A B: term n} :
+  Γ ⊢(Sc) t : A -> Γ ⊢(Sc) t : B -> A ≅ B.
+Proof.
+  induction 1 in B |- *.
+  - intro H'. apply typ_star_inv in H'. apply Requiv_sym. assumption.
+  - intro H'. apply typ_var_inv in H'. apply Requiv_sym. assumption.
+  - intro H'. apply typ_pi_inv in H' as [s0 [s'0 [Bequiv [typA [typB0 pi_check']]]]].
+    specialize (IHtyping2 _ typB0). apply srt_equiv_srt in IHtyping2. subst.
+    apply Requiv_sym. assumption.
+  - intro H'. apply typ_abs_inv in H' as [s0 [s0' [B' [S [Bequiv H']]]]].
+    apply Requiv_sym. eapply Requiv_trans; try eassumption.
+    change (Pi A ?x) with (fill (PiR A Hole) x).
+    apply step_equiv_context. apply Requiv_sym. intuition eauto.
+  - intro H'. apply typ_app_inv in H' as [A' [B' [Bequiv H']]].
+    refine (Requiv_trans _ (Requiv_sym _)); try eassumption. apply bind_preserves_step_equiv.
+    destruct H' as [typA _]. apply IHtyping1 in typA. apply pi_equiv_pi in typA. tauto.
+  - intro. eauto using Requiv_trans, Requiv_sym.
+Qed.
+
+Lemma srt_typing {n Sc} {Γ t} {T: term n} :
+  Γ ⊢(Sc) t : T -> T = Srt Box \/ (exists s, Γ ⊢(Sc) T: Srt s).
+Proof.
+  induction 1; auto.
+  - right. induction H; simpl.
+    + destruct (Nat.nlt_0_r _ _).
+    + destruct (lt_dec _ _).
+      * destruct (IHctx_wf (exist _ (proj1_sig i) l)) as [s'].
+        exists s'. change (Srt s') with (@ren n _ weaken (Srt s')). eapply weakening; try eassumption.
+      * exists s. change (Srt s) with (@ren n _ weaken (Srt s)). eapply weakening; try eassumption.
+  - destruct s'.
+    + right. exists Box. constructor. eapply typing_imp_ctx_wf. eassumption.
+    + left. constructor.
+  - right. exists s'. econstructor; try eassumption.
+  - destruct IHtyping1 as [|[s IHtyping1]]; try discriminate.
+    right. exists s.
+    apply typ_pi_inv in IHtyping1 as [s' [s'' [equiv_srts [typA [typB Sc_check]]]]].
+    apply srt_equiv_srt in equiv_srts. subst. rename s' into s, s'' into s'.
+    change (Srt s') with (bind (bind_first u) (Srt s')).
+    eapply bind_typ; try eassumption.
+    * intro. unfold bind_first at 1. simpl. rewrite bind_ren. rewrite bind_id.
+      { destruct (lt_dec _ _); try assumption. constructor. eauto using typing_imp_ctx_wf. }
+      clear. destruct k. unfold bind_first. simpl. destruct (lt_dec x n); try tauto.
+      f_equal. apply sig_lt_ext. reflexivity.
+    * eauto using typing_imp_ctx_wf.
+  - destruct IHtyping1.
+    + subst. apply srt_equiv in H0. left. clear IHtyping2. clear dependent t.
+      apply @no_spontaneous_srt_step_star with (K := Hole) in H0 as [k [K e]]. subst.
+      apply typed_imp_subterm_typed in H1 as [Γ' [T H]]. exfalso. revert H. clear.
+      remember (Srt Box). induction 1 in Heqt |- *; try discriminate; tauto.
+    + right. eauto.       
 Qed.
 
 Lemma preservation (Sc: pi_scheme) {n} Γ (t u : term n) A :
   Γ ⊢(Sc) t : A -> t ≻ u -> Γ ⊢(Sc) u : A.
 Proof.
   induction 1; intro red; inversion red; clear red;
-    match goal with H : fill ?K _ = _ _ |- _ => (destruct K; simpl in *; try discriminate;
-    subst; try solve [ match goal with H : _ [≻] _ |- _ => inversion H end ]) | _ => idtac end.
+    match goal with
+    | H : fill ?K _ = _ _ |- _ =>
+        (destruct K; simpl in *; try discriminate;
+         subst; try solve [ match goal with H : _ [≻] _ |- _ => inversion H end ])
+    | _ => idtac end.
   - inversion H2; subst; clear H2. econstructor; try eassumption.
     + apply IHtyping1. constructor. assumption.
     + eapply equiv_context; try eassumption.
       * simpl. intros. destruct (lt_dec _ _); try solve [constructor].
         apply ren_preserves_step_equiv. apply Requiv_clot_r. constructor. assumption.
+      * intros. simpl. destruct (lt_dec _ _).
+        -- assert (wfΓ : Γ ⊢(Sc)) by eauto using typing_imp_ctx_wf.
+           epose proof (Htyp := wf_ctx_contains_types wfΓ). destruct Htyp as [s0].
+           exists s0. change (@Srt (S ?n) ?x) with (ren weaken (@Srt n x)).
+           eapply weakening; eauto. apply IHtyping1. constructor. assumption.
+        -- exists s. change (@Srt (S ?n) ?x) with (ren weaken (@Srt n x)).
+           eapply weakening; eauto. apply IHtyping1. constructor. assumption.
       * econstructor; try eauto. { eapply typing_imp_ctx_wf. eassumption. } apply IHtyping1.
         constructor. assumption.
   - inversion H2; subst; clear H2. econstructor; try eassumption.
     apply IHtyping2. constructor. assumption.
-  - inversion H3; subst; clear H3. unshelve econstructor. { exact (Pi (fill K u0) B). }
+  - inversion H3; subst; clear H3. unshelve econstructor.
+    { exact (Pi (fill K u0) B). }
+    { exact s'. }
     + econstructor; try eauto.
       * apply IHtyping1. constructor. assumption.
       * eapply equiv_context; try eassumption.
         -- simpl. intros. destruct (lt_dec _ _); try solve [constructor].
            apply ren_preserves_step_equiv, Requiv_clot_r. constructor. assumption.
+        -- simpl. intros. destruct (lt_dec _ _).
+           ++ assert (wfΓ : Γ ⊢(Sc)) by eauto using typing_imp_ctx_wf.
+              epose proof (Htyp := wf_ctx_contains_types wfΓ). destruct Htyp as [s0].
+              exists s0. change (@Srt (S ?n) ?x) with (ren weaken (@Srt n x)).
+              eapply weakening; eauto. apply IHtyping1. constructor. assumption.
+           ++ exists s. change (@Srt (S ?n) ?x) with (ren weaken (@Srt n x)).
+              eapply weakening; eauto. apply IHtyping1. constructor. assumption.
         -- econstructor.
            ++ eapply typing_imp_ctx_wf; eassumption.
            ++ apply IHtyping1. constructor. assumption.
       * eapply equiv_context; try eassumption.
         -- simpl. intros. destruct (lt_dec _ _); try solve [constructor].
            apply ren_preserves_step_equiv, Requiv_clot_r. constructor. assumption.
+        -- simpl. intros. destruct (lt_dec _ _).
+           ++ assert (wfΓ : Γ ⊢(Sc)) by eauto using typing_imp_ctx_wf.
+              epose proof (Htyp := wf_ctx_contains_types wfΓ). destruct Htyp as [s0].
+              eexists. change (@Srt (S ?n) ?x) with (ren weaken (@Srt n x)).
+              eapply weakening; eauto. apply IHtyping1. constructor. assumption.
+           ++ eexists. change (@Srt (S ?n) ?x) with (ren weaken (@Srt n x)).
+              eapply weakening; eauto. apply IHtyping1. constructor. assumption.
         -- econstructor.
            ++ eapply typing_imp_ctx_wf; eassumption.
            ++ apply IHtyping1. constructor. assumption.
     + apply Requiv_clot_r. change (Pi (fill K ?x) B) with (fill (PiL K B) x). constructor.
       assumption.
+    + econstructor; eassumption.
   - inversion H3; subst; clear H3. econstructor; try eassumption.
     apply IHtyping3. constructor. assumption.
   - inversion H2; subst; clear H2. clear IHtyping1 IHtyping2.
     rename u0 into u.
-    apply typ_abs_inv in H. destruct H as [s [s' [B0 H]]].
-    destruct H as [Hequiv [type_ty [type_B0 [type_body pi_check]]]].
+    apply typ_abs_inv in H. destruct H as [s [s' [B0 [X H]]]].
+    destruct H as [Hequiv [type_ty [type_B0 [type_body [typ_piAB pi_check]]]]].
     apply pi_equiv_pi in Hequiv as [Aequiv Bequiv].
+    apply typ_pi_inv in typ_piAB as [s0 [s0' [Xequiv [typA [typB pi_check2]]]]].
     assert (true_type_body : Γ, ty ⊢(Sc) body : B).
-    { econstructor; eauto using Requiv_sym. }
+    { econstructor; eauto using Requiv_sym. eapply equiv_context; try eassumption.
+      - simpl. intros. apply ren_preserves_step_equiv.
+        destruct (lt_dec _ _); auto using Requiv_sym. constructor.
+      - simpl. intros. destruct (lt_dec k0 k).
+        +  edestruct (@wf_ctx_contains_types); swap 1 2.
+           * eexists x. change (@Srt (S ?n) ?x) with (ren weaken (@Srt n x)).
+             eapply weakening; try eassumption.
+           * eapply typing_imp_ctx_wf. eassumption.
+        + exists s0. change (@Srt (S ?n) ?x) with (ren weaken (@Srt n x)).
+          eapply weakening; try eassumption.
+      - econstructor; try eassumption. eapply typing_imp_ctx_wf; eassumption.
+    }
     assert (true_type_u : Γ ⊢(Sc) u : ty).
     { econstructor; eauto. }
     revert true_type_body true_type_u. clear. intros tybody tyu.
-    enough (
-        forall n k (σ : {i | i < k} -> term n) Γ Γ' x T,
-          (forall i, Γ ⊢(Sc) σ i : bind σ (kth_index_ctx Γ' (proj1_sig i) (proj2_sig i))) ->
-          Γ' ⊢(Sc) x : T -> Γ ⊢(Sc) -> Γ ⊢(Sc) bind σ x : bind σ T).
-    { eapply H; eauto using typing_imp_ctx_wf.
-      intro. destruct i; simpl. unfold bind_first at 1. simpl. destruct (lt_dec _ _).
-      - rewrite bind_ren. rewrite bind_id.
-        + constructor. eapply typing_imp_ctx_wf; eassumption.
-        + unfold bind_first, weaken. simpl. intro i. pose proof (proj2_sig i). simpl in *.
-          destruct (lt_dec _ _); try tauto. f_equal. apply sig_lt_ext. reflexivity.
-      - rewrite bind_ren. rewrite bind_id; try assumption.
-        unfold bind_first, weaken. simpl. intro i. pose proof (proj2_sig i). simpl in *.
+    eapply bind_typ; eauto using typing_imp_ctx_wf.
+    intro. destruct i; simpl. unfold bind_first at 1. simpl. destruct (lt_dec _ _).
+    + rewrite bind_ren. rewrite bind_id.
+      * constructor. eapply typing_imp_ctx_wf; eassumption.
+      * unfold bind_first, weaken. simpl. intro i. pose proof (proj2_sig i). simpl in *.
         destruct (lt_dec _ _); try tauto. f_equal. apply sig_lt_ext. reflexivity.
-    }
-    clear. intros ? ? ? ? ? ? ? H tyx Γwf. induction tyx in n, σ, Γ, H, Γwf |- *; simpl in *; auto.
-    + constructor. assumption.
-    + econstructor; eauto. eapply IHtyx2.
-      * intro. unfold lift_bind at 1. destruct (lt_dec _ _).
-        -- rewrite bind_weaken. eapply weakening.
-           ++ intro. simpl. pose proof (proj2_sig i0). destruct (lt_dec _ _); try tauto.
-              f_equal. f_equal. apply le_unique.
-           ++ apply H.
-           ++ econstructor; eauto.
-        -- rewrite bind_weaken.
-           replace (ren weaken (bind σ A)) with
-             (kth_index_ctx (Γ, bind σ A) n (Nat.lt_succ_diag_r n)).
-           ++ constructor. econstructor; eauto.
-           ++ simpl. destruct (lt_dec n n); try lia. reflexivity.
-      * econstructor; eauto.
-    + econstructor; eauto.
-      * apply IHtyx2.
-        -- intro. rewrite bind_weaken. unfold lift_bind.
-           destruct (lt_dec _ _).
-           ++ eapply weakening; eauto.
-              ** intro. simpl. pose proof (proj2_sig i0). simpl in *.
-                 destruct (lt_dec _ _); try tauto. f_equal. f_equal. apply le_unique.
-              ** econstructor; eauto.
-           ++ replace (ren weaken (bind σ A)) with
-                (kth_index_ctx (Γ, bind σ A) n (Nat.lt_succ_diag_r n)).
-              ** do 2 econstructor; eauto.
-              ** simpl. destruct (lt_dec _ _); try lia. reflexivity.
-        -- econstructor; eauto.
-      * apply IHtyx3.
-        -- intro. rewrite bind_weaken. unfold lift_bind at 1. destruct (lt_dec _ _).
-           ++ eapply weakening; eauto.
-              ** intro. simpl. pose proof (proj2_sig i0). simpl in *.
-                 destruct (lt_dec _ _); try tauto. f_equal. f_equal. apply le_unique.
-              ** econstructor; eauto.
-           ++ replace (ren weaken (bind σ A)) with
-                (kth_index_ctx (Γ, bind σ A) n (Nat.lt_succ_diag_r n)).
-              ** do 2 econstructor; eauto.
-              ** simpl. destruct (lt_dec _ _); try lia. reflexivity.
-        -- econstructor; eauto.
-    + rewrite bind_comp. replace (bind (bind σ ∘ bind_first u) B) with
-        (bind (bind_first (bind σ u)) (bind (lift_bind σ) B)).
-      * econstructor; eauto.
-      * rewrite bind_comp. apply bind_ext. intro. unfold lift_bind, bind_first at 2.
-        destruct (lt_dec _ _); simpl.
-        -- rewrite bind_ren. apply bind_id. intro. unfold weaken, bind_first. simpl.
-           pose proof (proj2_sig k). simpl in *. destruct (lt_dec _ _); try tauto.
-           f_equal. apply sig_lt_ext. reflexivity.
-        -- unfold bind_first. simpl. destruct (lt_dec _ _); try lia. reflexivity.
-    + econstructor; eauto. apply bind_preserves_step_equiv. assumption.
+    + rewrite bind_ren. rewrite bind_id; try assumption.
+      unfold bind_first, weaken. simpl. intro i. pose proof (proj2_sig i). simpl in *.
+      destruct (lt_dec _ _); try tauto. f_equal. apply sig_lt_ext. reflexivity.
   - inversion H1; subst; clear H1. econstructor; try eassumption.
     apply IHtyping1. constructor. assumption.
-  - inversion H1; subst; clear H1. econstructor.
+  - inversion H1; subst; clear H1. apply srt_typing in H as typPi.
+    destruct typPi as [|[s typPi]]; try discriminate.
+    apply typ_pi_inv in typPi as [s' [s0 [sequiv [typA [typB PiCheck]]]]].
+    apply srt_equiv_srt in sequiv. subst.
+    econstructor.
     + econstructor; try eassumption. apply IHtyping2. constructor. assumption.
     + apply bind_preserves_step_equiv_in_subs. intro. unfold bind_first.
       destruct (lt_dec _ _).
       * constructor.
       * apply Requiv_clot_r. constructor. assumption.
-  - subst. econstructor; try eassumption. apply IHtyping. constructor. assumption.
+    + change (Srt ?x) with (bind (bind_first (fill K t0)) (Srt x)).
+      eapply bind_typ; eauto using typing_imp_ctx_wf. simpl. intro. rewrite bind_ren.
+      rewrite bind_id.
+      * unfold bind_first. destruct (lt_dec _ _); try eassumption.
+        constructor. eapply typing_imp_ctx_wf. eassumption.
+      * intro. unfold bind_first, weaken. simpl. pose proof (proj2_sig k0). simpl in *.
+        destruct (lt_dec _ _); try tauto. f_equal. apply sig_lt_ext. reflexivity.
+  - subst. econstructor; try eassumption. apply IHtyping1. constructor. assumption.
 Qed.
 
 Lemma subject_reduction (Sc: pi_scheme) {n} Γ (t u : term n) A :
